First steps to use terminating closures of functional schemes

Multiplication.thy
@@ -2,20 +2,27 @@ theory Multiplication
 imports "IsaLibs/IsaLibs"
 begin
 
+declare[[
+  max_time_in_counter_ex = 4,
+  max_time_in_fitness = 50]]
+
 section {* Multiplication on Natural Numbers *}
 
 text {* This theory file shows how to find a function that multiplies natural numbers in Isabelle/HOL *}
 
 text {* We first define the functional space.*}
 
-definition scheme where
-"scheme P Q R S \<equiv> \<exists>(f::nat\<Rightarrow>nat\<Rightarrow>nat) (g::nat\<Rightarrow>nat\<Rightarrow>nat). \<forall>(x::nat) (y::nat).
-  ((f 0 y = P y Suc (0::nat)) \<and>
-   (f (Suc x) y = Q x y Suc (0::nat) (f x y)) \<and>
-   (g 0 y = R y Suc (0::nat)) \<and>
-   (g (Suc x) y = S x y Suc (0::nat) (f y) (g x y)))"
+definition scheme_const where
+"scheme_const M N \<equiv> \<exists>(f::nat\<Rightarrow>nat\<Rightarrow>nat) (g::nat\<Rightarrow>nat\<Rightarrow>nat). \<forall>(x::nat) (y::nat).
+  ((f 0 y = y) \<and>
+   (f (Suc x) y = M x y Suc (0::nat) (f x)) \<and>
+   (g 0 y = 0) \<and>
+   (g (Suc x) y = N x y Suc (0::nat) f (g x)))"
 
-thm scheme_def
+definition scheme_dest where
+"scheme_dest M N \<equiv> \<exists>(f::nat\<Rightarrow>nat\<Rightarrow>nat) (g::nat\<Rightarrow>nat\<Rightarrow>nat). \<forall>(x::nat) (y::nat).
+  ((f x y = M x y (0::nat) (\<lambda>x. x - (1::nat)) (\<lambda>x y z. if x then (y::nat) else z) (op = :: nat\<Rightarrow>nat\<Rightarrow>bool) f) \<and>
+   (g x y = N x y (0::nat) (\<lambda>x. x - (1::nat)) (\<lambda>x y z. if x then (y::nat) else z) (op = :: nat\<Rightarrow>nat\<Rightarrow>bool) f g))"
 
 text {* We then define the fitness function as the quadratic error, the termination criterion,
   and other GP related parameters. The function we want to synthesise multiplication in terms of 
@@ -24,71 +31,78 @@ text {* We then define the fitness function as the quadratic error, the terminat
 
 ML {*
   fun fitness ctxt consts =
-    let fun goal x y = x * y
+    let val in_out = [(@{term "0::nat"}, @{term "0::nat"} ,@{term "0::nat"}),
+                      (@{term "1::nat"}, @{term "1::nat"} ,@{term "1::nat"}),
+                      (@{term "2::nat"}, @{term "2::nat"} ,@{term "4::nat"}),
+                      (@{term "2::nat"}, @{term "3::nat"} ,@{term "6::nat"}),
+                      (@{term "3::nat"}, @{term "2::nat"} ,@{term "6::nat"}),
+                      (@{term "3::nat"}, @{term "3::nat"} ,@{term "9::nat"}),
+                      (@{term "2::nat"}, @{term "4::nat"} ,@{term "8::nat"}),
+                      (@{term "4::nat"}, @{term "2::nat"} ,@{term "8::nat"}),
+                      (@{term "3::nat"}, @{term "4::nat"} ,@{term "12::nat"}),
+                      (@{term "4::nat"}, @{term "4::nat"} ,@{term "16::nat"})]
         val f = consts (* |> tap (map (tracing o fst)) *)
-                       |> hd o tl
+                       |> hd
                        |> Const
-        val xs = 0 upto 9
-        val xs' = 1 upto (Utils.binomial_coefficient 10 2 - 1)
-                    |> map (Utils.choose xs 2)
-                    |> map (fn l => case l of
-                                      [x,y] => (x,y)
-                                    | _ => raise ERROR "")
-        val ys = map (fn (x,y) => goal x y) xs'
-        val rs = map (fn (x,y) => (f $ Utils.numeral_of_nat ctxt x $ Utils.numeral_of_nat ctxt y)
-                                |> (fn t => @{term "num_of_nat"} $ t)
-                                |> Value.value ctxt
-                                |> (fn t => @{term "numeral :: num\<Rightarrow>nat"} $ t)
-                                |> Utils.int_of_numeral) xs'
-        val ds = map2 (fn x => fn y => (x - y) * (x - y)) ys rs
-    in (0, ds) |> Library.foldl (op +)
-               |> Rat.rat_of_int end
+        val conjectures =
+          in_out |> map (fn (x,y,r) => (f $ x $ y, r) |> HOLogic.mk_eq
+                                                      |> HOLogic.mk_Trueprop)
+(*                 |> tap (map (tracing o Syntax.string_of_term ctxt))*)
+        val ctxt = Local_Theory.target_of ctxt
+        val error = conjectures |> map (Counter_Example.counter_example ctxt 10)
+                                |> map (fn foo => if foo then 1 else 0)
+    in (0, error) |> Library.foldl (op +)
+(*                  |> tap (tracing o string_of_int)*)
+                  |> Rat.rat_of_int end
   fun finish ({fit, ...} : GP.individual) = Rat.eq (Rat.zero, fit)
   fun test ctxt consts =
       consts |> fitness ctxt
              |> pair Rat.zero
              |> Rat.eq
-  val term_size = 13
-  val population_size = 100
+  val term_size = 20
+  val population_size = 200
   val generations = 100
   val bests = 10
   val mut_prob = 0.05
-  val scheme = @{thm "scheme_def"}
+  val scheme_dest = @{thm "scheme_dest_def"}
+  val scheme_const = @{thm "scheme_const_def"}
+  val experiments = 20
 *}
 
 text {* We finally call the GP algorithm. *}
 
 (*local_setup {*
  fn lthy => 
-  case DB_EXHAUST.exhaust true lthy scheme term_size [] test of
-    SOME (ctxt, t, trms) => 
-      let val _ = map (tracing o (Syntax.string_of_term ctxt)) trms
-      in ctxt end
-  | NONE => lthy
+  let val Const C = @{term "op * :: nat\<Rightarrow>nat\<Rightarrow>nat"}
+      val ff = fitness lthy [C, C]
+      val _ = tracing (Rat.string_of_rat ff)
+  in lthy end
 *}*)
 
 local_setup {*
  fn lthy => 
-  case GP.evolve false scheme lthy fitness finish term_size population_size generations bests mut_prob of
-    SOME ind => (#ctxt ind)
-  | NONE => lthy
+    let 
+        val sts2 =
+      1 upto experiments
+        |> map (fn _ => GP.evolve true false scheme_dest lthy fitness finish
+                                  term_size population_size generations bests mut_prob)
+        val (eqs2, alleq2) = GNU_Plot.gp_statistics_to_equals population_size sts2
+        val _ = tracing ("gp_statistics_to_equals Destructive: (" ^ string_of_int eqs2 ^ ", " ^ string_of_int alleq2 ^ ")")
+        val (nt2, allnt2) = GNU_Plot.gp_statistics_to_non_terminating sts2
+        val _ = tracing ("gp_statistics_to_non_terminating Destructive: (" ^ string_of_int nt2 ^ ", " ^ string_of_int allnt2 ^ ")")
+        val _ = GNU_Plot.gp_statistics_to_error_plot "MulDest" generations sts2
+val sts1 =
+      1 upto experiments
+        |> map (fn _ => GP.evolve true false scheme_const lthy fitness finish
+                                  term_size population_size generations bests mut_prob)
+        val (eqs1, alleq1) = GNU_Plot.gp_statistics_to_equals population_size sts1
+        val _ = tracing ("gp_statistics_to_equals Constructive: (" ^ string_of_int eqs1 ^ ", " ^ string_of_int alleq1 ^ ")")
+        val (nt1, allnt1) = GNU_Plot.gp_statistics_to_non_terminating sts1
+        val _ = tracing ("gp_statistics_to_non_terminating Constructive: (" ^ string_of_int nt1 ^ ", " ^ string_of_int allnt1 ^ ")")
+        val _ = GNU_Plot.gp_statistics_to_error_plot "SumConsts" generations sts1
+
+        val _ = GNU_Plot.gp_statistics_to_cumulative_prob_plot "Mul" generations sts1 sts2
+    in lthy end
 *}
-
-text {* Genome is composed by: 
-@{term "\<lambda>x xa xb xc xd. xd"}
-@{term "\<lambda>x xa xb. xb"}
-@{term "\<lambda>x xa xb xc. xb"}
-@{term "\<lambda>x xa xb. x"} *}
-
-thm f.simps
-thm g.simps
-
-text {* Invented functions are well-defined *}
-lemma "scheme (\<lambda>x xa xb. x) (\<lambda>x xa xb xc. xb) (\<lambda>x xa xb. xb) (\<lambda>x xa xb xc xd. xd)"
-apply (unfold scheme_def)
-apply (rule_tac x="f" in exI)
-apply (rule_tac x="g" in exI)
-apply simp
-done
 
 end
